theories/lang/cpp/logic/destroy.v
@@ -59,11 +59,11 @@ Section destroy.
 
      TODO we can remove [dtor] with the new destructor scheme
    *)
-  Fixpoint destruct_val (dispatch : bool) (t : type) (this : ptr) (dtor : option obj_name) (Q : mpred)
+  Fixpoint destruct_val (dispatch : bool) (t : type) (this : ptr) (Q : mpred)
            {struct t}
   : mpred :=
     match t with
-    | Tqualified _ t => destruct_val dispatch t this dtor Q
+    | Tqualified _ t => destruct_val dispatch t this Q
     | Tnamed cls =>
       match σ.(genv_tu) !! cls with
       | Some (Gstruct s) =>
@@ -101,14 +101,14 @@ Section destroy.
     | Tarray t sz =>
       (* NOTE when destroying an array, elements of the array are destroyed with non-virtual dispatch. *)
       fold_right (fun i Q => valid_ptr (this .[ t ! Z.of_nat i ]) **
-         destruct_val false t (this .[ t ! Z.of_nat i ]) dtor Q) Q (List.rev (seq 0 (N.to_nat sz)))
+         destruct_val false t (this .[ t ! Z.of_nat i ]) Q) Q (List.rev (seq 0 (N.to_nat sz)))
     | _ =>
       (* |={↑pred_ns}=> *) this |-> anyR (erase_qualifiers t) 1 ** (this |-> tblockR (erase_qualifiers t) 1 -* Q)
       (* emp *)
     end%I.
 
-  Lemma destruct_val_frame dispatch : forall ty this dt Q Q',
-      Q -* Q' |-- destruct_val dispatch ty this dt Q -* destruct_val dispatch ty this dt Q'.
+  Lemma destruct_val_frame dispatch : forall ty this Q Q',
+      Q -* Q' |-- destruct_val dispatch ty this Q -* destruct_val dispatch ty this Q'.
   Proof.
     intro ty; generalize dependent dispatch; induction ty; simpl; eauto;
       try solve [
